Listing imports and exports.

lib/prelude/consistency.bpl
@@ -1,7 +1,22 @@
-// ---------- Representation of linearization
+/**
+ * Imported declarations
+ */
+
+// type Invoc;
+// type SeqInvoc;
+// type SetInvoc;
+
+/**
+ * Exported declarations
+ */
+
+// hb(x, y) : x happens-before y.
+// We assume there exists such a function, given by the client program
+function hb(x: Invoc, y: Invoc): bool;
+axiom (forall n: Invoc :: !hb(n, n));
 
 // A shared global variable that builds the linearization
 var {:layer 1,2} lin: SeqInvoc;
 
 // A map from invocations to the set of prior invocations visible to them
-var {:layer 1,2} vis: [Invoc]SetInvoc;
+var {:layer 1,2} vis: [Invoc] SetInvoc;
